@prefix rdf: <http://www.w3.org/1999/02/22-rdf-syntax-ns#> .
@prefix owl: <http://www.w3.org/2002/07/owl#> .
@prefix rdfs: <http://www.w3.org/2000/01/rdf-schema#> .
@prefix sosa: <http://www.w3.org/ns/sosa/> .
@prefix geosparql: <http://www.opengis.net/ont/geosparql#> .
@prefix xsd: <http://www.w3.org/2001/XMLSchema#> .
@prefix geo: <http://www.w3.org/2003/01/geo/wgs84_pos#> .
@prefix dct: <http://purl.org/dcterms/terms/> .
@prefix skos: <http://www.w3.org/2004/02/skos/core#> .
@prefix ssn: <http://www.w3.org/ns/ssn/> .
@prefix time: <http://www.w3.org/2006/time#> .

<http://ns.inria.fr/meteo/ontology/WeatherStation>
  a owl:Class ;
  rdfs:subclassof sosa:Platform, <http://www.opengis.net/ont/geosparql#Feature> ;
  geosparql:hasGeometry [
    a geosparql:Geometry ;
    geosparql:asWKT geosparql:wktLiteral
  ] ;
  rdfs:label "Station Meteo"@fr ;
  geo:lat xsd:double ;
  geo:long xsd:double ;
  geo:alt xsd:int ;
  dct:spatial <http://www.wikidata.org/entity/Q2221906> .

<http://ns.inria.fr/meteo/ontology/WeatherProperty>
  a owl:Class, rdfs:Class ;
  rdfs:label "Weather Property"@en ;
  #skos:definition "An observable quality (property, characteristic) of a meterological feature of interest. A weather property can be measured (e.g. wind speed) or observed (cloud cover)"@en ;
  rdfs:subClassOf sosa:ObservableProperty, ssn:Property ;
  owl:equivalentClass [
    a owl:Restriction ;
    owl:onProperty ssn:isPropertyOf ;
    owl:qualifiedCardinality "1"^^xsd:int ;
    owl:onClass <http://ns.inria.fr/meteo/ontology/MeteorologicalFeature>
  ] ;
  rdfs:comment " A weather Property is an observable property of exactly one Meterological feature."@en .

<http://ns.inria.fr/meteo/ontology/MeteorologicalFeature>
  a owl:Class, rdfs:Class ;
  rdfs:label "Meteorological Feature"@en ;
  owl:equivalentClass[ owl:intersectionOf (sosa:FeatureOfInterest 
  [ a owl:Restriction; owl:onProperty ssn:hasProperty; owl:allValuesFrom weo:WeatherProperty] 
  [ a owl:Restriction; owl:onProperty ssn:hasProperty; owl:minCardinality "1"^^xsd:int]) ];
  skos:definition "The meteorological phenomenon whose property is being measured or observed in the course of an Observation."@en ;
  rdfs:comment "For each Meteorological feature such as wind or precipitations, at least one property (precipitation amount) need to be defined "@en .

<http://ns.inria.fr/meteo/ontology/MeteorologicalObservation>
  a owl:Class ;
  owl:equivalentClass [ owl:intersectionOf (sosa:Observation 
  [ a owl:Restriction ; owl:onProperty sosa:observedProperty ; owl:allValuesFrom weo:WeatherProperty] 
  [ a owl:Restriction ; owl:onProperty sosa:hasFeatureOfInterest; owl:allValuesFrom weo:MeteorologicalFeature])];
  rdfs:label "Meterological Observation"@en ;
  skos:definition "Act of carrying out a procedure to estimate a value of a property of a Meterological feature."@en ;
  rdfs:comment " meterological observation is an observation which is linked to exactly one weather property and one meteorological feature."@en .

<http://ns.inria.fr/meteo/ontology/Interval3h>
  a owl:Class ;
  owl:equivalentClass [ owl:intersectionOf (time:Interval 
    [ a owl:Restriction ;
      owl:onProperty time:hasDuration ;
      owl:allValuesFrom [ owl:intersectionOf(
      time:Duration 
      [ a owl:Restriction ; owl:onProperty time:numericDuration  ; owl:hasValue 3.0 ]
      [ a owl:Restriction ; owl:onProperty time:unitType  ; owl:hasValue time:unitHour ] )
      
    ])
  ] .

<http://ns.inria.fr/meteo/ontology/Interval24h>
  a owl:Class ;
  rdfs:subClassOf time:Interval ;
  owl:equivalentClass [
    a owl:Restriction ;
    owl:onProperty time:hasDuration ;
    owl:hasValue [
      a time:Duration ;
      time:numericDuration 24.0 ;
      time:unitType time:unitHour
    ]
  ] .

<http://ns.inria.fr/meteo/ontology/Interval10min>
  a owl:Class ;
  rdfs:subClassOf time:Interval ;
  owl:equivalentClass [
    a owl:Restriction ;
    owl:onProperty time:hasDuration ;
    owl:hasValue [
      a time:Duration ;
      time:numericDuration 10.0 ;
      time:unitType time:unitMinute
    ]
  ] .

<http://ns.inria.fr/meteo/ontology/property/madeByStation>
  a owl:ObjectProperty ;
  rdfs:domain <http://ns.inria.fr/meteo/ontology/WeatherStation> ;
  rdfs:range <http://ns.inria.fr/meteo/ontology/MeteorologicalObservation> .
 

<http://ns.inria.fr/meteo/ontology/property/stationID>
  a owl:DatatypeProperty ;
  rdfs:domain <http://ns.inria.fr/meteo/ontology/WeatherStation> .

<http://ns.inria.fr/meteo/ontology/property/hasAbbreviation>
  a owl:DatatypeProperty ;
  rdfs:range <http://ns.inria.fr/meteo/ontology/WeatherProperty> .