@prefix time:           <http://www.w3.org/2006/time#> .
@prefix qb4st:          <http://resources.opengeospatial.org/def/qbcomponents/qb4st> .
@prefix rdf:            <http://www.w3.org/1999/02/22-rdf-syntax-ns#> .
@prefix rdfs:           <http://www.w3.org/2000/01/rdf-schema#> .
@prefix owl:            <http://www.w3.org/2002/07/owl#> .
@prefix xsd:            <http://www.w3.org/2001/XMLSchema#> .
@prefix skos:           <http://www.w3.org/2004/02/skos/core#> .
@prefix qb:             <http://purl.org/linked-data/cube#> .
@prefix wes-dimension:  <http://ns.inria.fr/meteo/observationslice/dimension#> .
@prefix wes-attribute:  <http://ns.inria.fr/meteo/observationslice/attribute#> .
@prefix wes-measure:    <http://ns.inria.fr/meteo/observationslice/measure#> .
@prefix wes:            <http://ns.inria.fr/meteo/observationslice/>  .
@prefix wevp:           <http://ns.inria.fr/meteo/vocab/weatherproperty/> .
@prefix weo:            <http://ns.inria.fr/meteo/ontology/> . 
@prefix dct:            <http://purl.org/dc/terms/> .

<http://ns.inria.fr/meteo/dataset-MF/2021> a qb:DataSet;
qb:structure wes:annualTimeSeries;
dct:description "RDF French Weather Dataset for 2021 uplifted and aggregated from Meteo-France Open Data Archives"@en.

<http://ns.inria.fr/meteo/dataset-MF/2020> a qb:DataSet;
qb:structure wes:annualTimeSeries;
dct:description "French Weather Dataset for 2020 uplifted and aggregated from Meteo-France Open Data Archives"@en.

<http://ns.inria.fr/meteo/dataset-MF/2019> a qb:DataSet;
qb:structure wes:annualTimeSeries;
dct:description "French Weather Dataset for 2019 uplifted and aggregated from Meteo-France Open Data Archives"@en.

<http://ns.inria.fr/meteo/dataset-MF/2018> a qb:DataSet;
qb:structure wes:annualTimeSeries;
dct:description "French Weather Dataset for 2018 uplifted and aggregated from Meteo-France Open Data Archives"@en.

<http://ns.inria.fr/meteo/dataset-MF/2017> a qb:DataSet;
qb:structure wes:annualTimeSeries;
dct:description "French Weather Dataset for 2017 uplifted and aggregated from Meteo-France Open Data Archives"@en.

<http://ns.inria.fr/meteo/dataset-MF/2016> a qb:DataSet;
qb:structure wes:annualTimeSeries;
dct:description "French Weather Dataset for 2016 uplifted and aggregated from Meteo-France Open Data Archives"@en.

wes:annualTimeSeries a qb:DataStructureDefinition, qb4st:SpatioTemporalDSD; 
    qb:component 
        [qb:dimension wes-dimension:station; qb:order 1; qb:componentAttachment qb:Slice],
        [qb:dimension wes-dimension:year; qb:order 2; qb:componentAttachment qb:Slice],
        [qb:measure wes-measure:minDailyTemperature],  
        [qb:measure wes-measure:maxDailyTemperature], 
        [qb:measure wes-measure:avgDailyTemperature],
        [qb:measure wes-measure:rainfall24h],
        [qb:attribute wes-attribute:Date; qb:componentAttachment qb:Slice];
        qb:sliceKey wes:SliceByStationAndYear .

wes:sliceByStationAndYear a qb:SliceKey;
    rdfs:label "Meterological observations sliced by weather station and by year"@en;
    rdfs:comment "Meterological Data slice by grouping meterological observations of the same station together by year"@en;
    qb:componentProperty wes-dimension:station, wes-dimension:year .

wes-dimension:station a rdf:Property, qb:DimensionProperty; 
    rdfs:label "a weather station as a spatial dimension";
    rdfs:subPropertyOf sdmx-dimension:refArea ;
    rdfs:range weo:WeatherStation. 

wes-dimension:year a rdf:Property, qb:DimensionProperty; 
    rdfs:label "a year as a temporal dimension";
    rdfs:subPropertyOf sdmx-dimension:refPeriod ;
    rdfs:range xsd:gYear.

wes-measure:minDailyTemperature a rdf:Property, qb:MeasureProperty; 
    rdfs:label "Minimum Daily Temperature in Celsius"@en;
    sdmx-attribute:unitMeasure <http://qudt.org/vocab/unit/DEG_C>  ; 
    rdfs:range xsd:decimal ;
    qb:concept wevp:airTemperature . 

wes-measure:maxDailyTemperature a rdf:Property, qb:MeasureProperty; 
    rdfs:label "Maximum Daily Temperature in Celsius"@en;
    sdmx-attribute:unitMeasure <http://qudt.org/vocab/unit/DEG_C>  ; 
    rdfs:range xsd:decimal ;
    qb:concept wevp:airTemperature .

wes-measure:avgDailyTemperature a rdf:Property, qb:MeasureProperty; 
    rdfs:label "Mean Daily Temperature in Celsius"@en;
    sdmx-attribute:unitMeasure <http://qudt.org/vocab/unit/DEG_C>  ; 
    rdfs:range xsd:decimal ; 
    qb:concept wevp:airTemperature .

wes-measure:rainfall24h a rdf:Property, qb:MeasureProperty; 
    rdfs:label "Cumulative Rainfall during 24h"@en;
    sdmx-attribute:unitMeasure <http://qudt.org/vocab/unit/MilliM>  ; 
    rdfs:range xsd:decimal ; 
    qb:concept wevp:precipitationAmount .



