@prefix rdf: <http://www.w3.org/1999/02/22-rdf-syntax-ns#> .
@prefix owl: <http://www.w3.org/2002/07/owl#> .
@prefix rdfs: <http://www.w3.org/2000/01/rdf-schema#> .
@prefix sosa: <http://www.w3.org/ns/sosa/> .
@prefix geosparql: <http://www.opengis.net/ont/geosparql#> .
@prefix xsd: <http://www.w3.org/2001/XMLSchema#> .
@prefix geo: <http://www.w3.org/2003/01/geo/wgs84_pos#> .
@prefix dcterms: <http://purl.org/dcterms/terms/> .
@prefix skos: <http://www.w3.org/2004/02/skos/core#> .
@prefix ssn: <http://www.w3.org/ns/ssn/> .
@prefix time: <http://www.w3.org/2006/time#> .

<http://ns.inria.fr/meteo/ontology/WeatherStation>
  a owl:Class ;
  rdfs:subclassof sosa:Platform, <http://www.opengis.net/ont/geosparql#Feature> ;
  geosparql:hasGeometry [
    a geosparql:Geometry ;
    geosparql:asWKT geosparql:wktLiteral
  ] ;
  rdfs:label xsd:string ;
  geo:lat xsd:double ;
  geo:long xsd:double ;
  geo:alt xsd:int ;
  dcterms:spatial <http://www.wikidata.org/entity/Q2221906> .

<http://ns.inria.fr/meteo/ontology/WeatherProperty>
  a owl:Class, rdfs:Class ;
  rdfs:label "Weather Property"@en ;
  skos:definition "An observable quality (property, characteristic) of a meterological feature of interest. A weather property can be measured (e.g. wind speed) or observed (cloud cover)"@en ;
  rdfs:subClassOf sosa:ObservableProperty, ssn:Property ;
  owl:equivalentClass [
    a owl:Restriction ;
    owl:onProperty ssn:isPropertyOf ;
    owl:QualifiedCardinality "1"^^xsd:int ;
    owl:onClass <http://ns.inria.fr/meteo/ontology/MeteorologicalFeature>
  ] ;
  rdfs:comment "This class is used to represent all weather parameters covered by Meteo France SYNOP reports."@en .

<http://ns.inria.fr/meteo/ontology/MeteorologicalFeature>
  a owl:Class, rdfs:Class ;
  rdfs:label "Meteorological Feature"@en ;
  rdfs:subClassOf sosa:FeatureOfInterest ;
  skos:definition "The meteorological phenomenon whose property is being measured or observed in the course of an Observation."@en ;
  owl:equivalentClass [
    a owl:Restriction ;
    owl:onProperty ssn:hasProperty ;
    owl:minQualifiedCardinality "1"^^xsd:int ;
    owl:onClass <http://ns.inria.fr/meteo/ontology/WeatherProperty>
  ] ;
  rdfs:comment "For each Meteorological feature such as wind or precipitations, at least one property (precipitation amount) need to be defined "@en .

<http://ns.inria.fr/meteo/ontology/MeteorologicalObservation>
  a owl:Class ;
  rdfs:subClassOf sosa:Observation, [
    a owl:Restriction ;
    owl:onProperty sosa:observedProperty ;
    owl:allValuesFrom <http://ns.inria.fr/meteo/ontology/WeatherProperty>
  ];
  rdfs:label "Meterological Observation" ;
  skos:definition "Act of carrying out a procedure to estimate a value of a property of a Meterological feature."@en ;
  rdfs:comment "A meterological observation is an observation which is linked to one unique weather property."@en .

<http://ns.inria.fr/meteo/ontology/Interval3h>
  a owl:Class ;
  rdfs:subClassOf time:Interval ;
  owl:equivalentClass [
    a owl:Restriction ;
    owl:onProperty time:hasDuration ;
    owl:hasValue [
      a time:Duration ;
      time:numericDuration 3.0 ;
      time:unitType time:unitHour
    ]
  ] .

<http://ns.inria.fr/meteo/ontology/Interval24h>
  a owl:Class ;
  rdfs:subClassOf time:Interval ;
  owl:equivalentClass [
    a owl:Restriction ;
    owl:onProperty time:hasDuration ;
    owl:hasValue [
      a time:Duration ;
      time:numericDuration 24.0 ;
      time:unitType time:unitHour
    ]
  ] .

<http://ns.inria.fr/meteo/ontology/Interval10min>
  a owl:Class ;
  rdfs:subClassOf time:Interval ;
  owl:equivalentClass [
    a owl:Restriction ;
    owl:onProperty time:hasDuration ;
    owl:hasValue [
      a time:Duration ;
      time:numericDuration 10.0 ;
      time:unitType time:unitMinute
    ]
  ] .

<http://ns.inria.fr/meteo/ontology/property/madeByStation>
  a owl:ObjectProperty ;
  rdfs:domain <http://ns.inria.fr/meteo/ontology/WeatherStation> ;
  rdfs:range <http://ns.inria.fr/meteo/ontology/MeteorologicalObservation> .
 

<http://ns.inria.fr/meteo/ontology/property/stationID>
  a owl:DatatypeProperty ;
  rdfs:domain <http://ns.inria.fr/meteo/ontology/WeatherStation> ;
  rdfs:range xsd:string .

<http://ns.inria.fr/meteo/ontology/property/hasAbbreviation>
  a owl:DatatypeProperty ;
  rdfs:range <http://ns.inria.fr/meteo/ontology/WeatherProperty> ;
  rdfs:domain xsd:string .